refina a int insertion sort

InsertionSort.fst
@@ -1,46 +1,44 @@
 module InsertionSort
 
-type ord a = f:(a -> a -> bool){forall x y. not (f x y) ==> f x y}
-
-let rec count (#a: eqtype) (x:a) (l:list a) : nat =
+let rec count (x:int) (l:list int) : nat =
   match l with
     | [] -> 0
     | y::l' -> (if x = y then 1 else 0) + count x l'
 
-let perm (#a: eqtype) (l1 l2: list a) : GTot Type =
-  forall (x:a). count x l1 == count x l2
+let perm (l1 l2: list int) : GTot Type =
+  forall (x:int). count x l1 == count x l2
 
-let rec sorted (#a:eqtype) (leq: ord a) (xs: list a) : bool =
+let rec sorted  (xs: list int) : bool =
   match xs with
     | []
     | [_] -> true
-    | x::y::l' -> leq x y && sorted leq (y::l')
+    | x::y::l' ->  x <= y && sorted (y::l')
 
-let rec insert (#a:eqtype) (leq: ord a) (x:a) (l:list a) : list a =
+let rec insert (x: int) (l:list int) : list int =
   match l with
     | [] -> [x]
     | y::l' ->
-      if leq x y
+      if x <= y
       then x::l
-      else y :: (insert leq x l')
+      else y :: (insert x l')
 
-let rec lem_insert_perm (#a:eqtype) (leq: ord a) x l
-  : Lemma (perm (x::l) (insert leq x l))
+let rec lem_insert_perm x l
+  : Lemma (perm (x::l) (insert x l))
 = match l with
     | [] -> ()
-    | y::l' -> lem_insert_perm leq x l'
+    | y::l' -> lem_insert_perm x l'
 
-let rec lem_insert_sorted (#a:eqtype) (leq: ord a) x l
-  : Lemma (requires sorted leq l) (ensures sorted leq (insert leq x l))
+let rec lem_insert_sorted x l
+  : Lemma (requires sorted l) (ensures sorted (insert x l))
 = match l with
     | [] -> ()
-    | y::l' -> lem_insert_sorted leq x l'
+    | y::l' -> lem_insert_sorted x l'
 
-let rec insertion_sort (#a:eqtype) (leq: ord a) (xs: list a) :
-  xs':(list a){perm xs xs' /\ sorted leq xs'}
+let rec insertion_sort (xs: list int) :
+  xs':(list int){perm xs xs' /\ sorted xs'}
 = match xs with
     | [] -> []
     | x::xs ->
-      lem_insert_perm leq x (insertion_sort leq xs);
-      lem_insert_sorted leq x (insertion_sort leq xs);
-      insert leq x (insertion_sort leq xs)
+      lem_insert_perm x (insertion_sort xs);
+      lem_insert_sorted x (insertion_sort xs);
+      insert x (insertion_sort xs)
